src/Soundness.v
@@ -12,17 +12,52 @@ Module Soundness (P : PAT).
 
     Lemma ok_term_Topen_push :
       forall Gamma T t t' ty,
-      Gamma & T ~ BindTName |= Topen_t 0 (FTName T) t ~: ty ->
-      push_value TmType t t' ->
-      Gamma |= t' ~: ty.
-    Admitted.
+        Gamma & T ~ BindTName |= Topen_t 0 (FTName T) t ~: ty ->
+        push_value TmType t t' ->
+        Gamma |= t' ~: ty.
+    Proof.
+      Admitted.
+      (* introv Htype Hpush. *)
+      (* remember TmType as f eqn:Hf. *)
+      (* induction Hpush ; substs. *)
+      (* - inverts Htype. *)
+      (*   assert (Topen_ty 0 (FTName T) ty0 = ty0) by admit. *)
+      (*   rewrite H in *. *)
+      (*   apply_fresh TLam as x. admit. *)
+      (*   (* apply_empty ok_type_tname_strengthening. *) *)
+      (*   simpls. apply_fresh TType as T'. *)
 
     Lemma ok_term_Kopen_push :
       forall Gamma K d ty' T t t' ty,
-      Gamma & K ~ BindCon d ty' T |= Kopen_t 0 (FCon K) t ~: ty ->
-      push_value (TmConDef d ty' T) t t' ->
-      Gamma |= t' ~: ty.
+        Gamma & K ~ BindCon d ty' T |= Kopen_t 0 (FCon K) t ~: ty ->
+        push_value (TmConDef d ty' T) t t' ->
+        Gamma |= t' ~: ty.
     Admitted.
+
+    Theorem preservation :
+      forall Gamma t t' ty,
+        Gamma |= t ~: ty ->
+        t --> t' ->
+        Gamma |= t' ~: ty.
+    Proof.
+      introv hasType Hstep.
+      gen t'.
+      induction hasType; intros; inverts Hstep ;
+        try (with_hyp (is_context _) as ctx ; with_hyp (_ = _) as eq
+             ; inverts ctx ; inverts* eq).
+      { Case "TmApp". inverts hasType1.
+        pick_fresh x. rewrite* (@subst_intro x).
+        apply_empty* ok_term_subst. }
+      { Case "TmTyApp". inverts hasType.
+        pick_fresh X.
+        rewrite* (@tsubst_intro X).
+        rewrite* (@tsubst_t_intro X).
+        apply_empty~ ok_term_tsubst. }
+      { Case "TmType". pick_fresh T'. applys* ok_term_Topen_push T'. }
+      { Case "TmTypeCong". apply_fresh TType as T' ; auto. }
+      { Case "TmConDef". pick_fresh K'. applys* ok_term_Kopen_push K'. }
+      { Case "TmConDefCong". apply_fresh TConDef as K'; auto. }
+    Qed.
 
     Definition no_vars (Gamma : env) : Prop :=
       forall x ty, binds x (BindVar ty) Gamma -> False.
@@ -45,46 +80,24 @@ Module Soundness (P : PAT).
         inverts Hval; inverts* hasType. }
       { Case "TmCon".
         forwards* [Hval | (t' & Hstep)]: IHhasType. }
-      Admitted.
-    (*   { Case "TmType". right. pick_fresh T. *)
-    (*     forwards* [Hval | (t' & Hstep)]: H1 T. *)
-    (*     + introv Hb. binds_cases Hb. apply* Hnv. *)
-    (*     + forwards* (v' & Hpush): Topen_push Hval. *)
-    (*     + forwards~ (t'0 & Heq) : Topen_step Hstep. rewrite* Heq in Hstep. } *)
-    (*   { Case "TmConDef". right. pick_fresh K. *)
-    (*     forwards* [Hval | (t' & Hstep)]: H4 K. *)
-    (*     + introv Hb. binds_cases Hb. apply* Hnv. *)
-    (*     + forwards* (v' & Hpush): Kopen_push Hval. *)
-    (*     + forwards (t'0 & Heq) : Kopen_step Hstep. rewrite* Heq in Hstep. } *)
-    (* Qed. *)
-
-    Theorem preservation :
-      forall Gamma t t' ty,
-        Gamma |= t ~: ty ->
-        t --> t' ->
-        Gamma |= t' ~: ty.
-    Proof.
-      introv hasType Hstep.
-      gen t'.
-      induction hasType; intros; inverts Hstep ;
-        try (with_hyp (is_context _) as ctx ; with_hyp (_ = _) as eq
-             ; inverts ctx ; inverts* eq).
-      { Case "TmApp". inverts hasType1.
-        pick_fresh x. rewrite* (@subst_intro x).
-        apply_empty* ok_term_subst. }
-      { Case "TmTyApp". inverts hasType.
-        pick_fresh X.
-        rewrite* (@tsubst_intro X).
-        rewrite* (@tsubst_t_intro X).
-        apply_empty~ ok_term_tsubst. }
-      { Case "TmType". pick_fresh T'.
-        applys* ok_term_Topen_push T'. }
-      { Case "TmTypeCong". apply_fresh TType as T' ; auto.
-        apply~ H1. apply* Topen_step_change. }
-      { Case "TmConDef". pick_fresh K'.
-        applys* ok_term_Kopen_push K'. }
-      { Case "TmConDefCong". apply_fresh TConDef as K'; auto.
-        apply~ H4. apply* Kopen_step_change. }
+      { Case "TmType". right. pick_fresh T.
+        forwards* [Hval | (t' & Hstep)]: H1 T.
+        + introv Hb. binds_cases Hb. apply* Hnv.
+        + forwards Hval' : Topen_is_value Hval.
+          forwards* (v' & Hpush): is_value_push Hval'.
+        + forwards (tclose & Heq): Topen_t_close 0 (FTName T) t'.
+          * forwards* ?: preservation Hstep.
+          * substs. eexists. apply_fresh ETypeCong.
+            apply* Topen_step_change. }
+      { Case "TmConDef". right. pick_fresh K.
+        forwards* [Hval | (t' & Hstep)]: H4 K.
+        + introv Hb. binds_cases Hb. apply* Hnv.
+        + forwards Hval' : Kopen_is_value Hval.
+          forwards* (v' & Hpush): is_value_push Hval'.
+        + forwards (tclose & Heq) : Kopen_t_close 0 (FCon K) t'.
+          * forwards* ?: preservation Hstep.
+          * substs. eexists. apply_fresh EConDefCong.
+            apply* Kopen_step_change. }
     Qed.
 
   End Soundness.
